proofs/hol_light/x86_64/proofs/mlkem_poly_compress_d11.ml
@@ -715,4 +715,288 @@ let mlkem_poly_compress_d11_mc =
 ];;
 (*** BYTECODE END ***)
 
-(* TODO: Prove correctness of poly_compress_d11_avx2 *)
+let mlkem_poly_compress_d11_tmc =
+  define_trimmed "mlkem_poly_compress_d11_tmc" mlkem_poly_compress_d11_mc;;
+let MLKEM_POLY_COMPRESS_D11_TMC_EXEC =
+  X86_MK_CORE_EXEC_RULE mlkem_poly_compress_d11_tmc;;
+
+(* ------------------------------------------------------------------------- *)
+(* Code length constants                                                     *)
+(* ------------------------------------------------------------------------- *)
+
+let LENGTH_MLKEM_POLY_COMPRESS_D11_MC =
+  REWRITE_CONV[mlkem_poly_compress_d11_mc] `LENGTH mlkem_poly_compress_d11_mc`
+  |> CONV_RULE (RAND_CONV LENGTH_CONV);;
+
+let LENGTH_MLKEM_POLY_COMPRESS_D11_TMC =
+  REWRITE_CONV[mlkem_poly_compress_d11_tmc] `LENGTH mlkem_poly_compress_d11_tmc`
+  |> CONV_RULE (RAND_CONV LENGTH_CONV);;
+
+let LENGTH_SIMPLIFY_CONV =
+  REWRITE_CONV[LENGTH_MLKEM_POLY_COMPRESS_D11_MC;
+               LENGTH_MLKEM_POLY_COMPRESS_D11_TMC] THENC
+  NUM_REDUCE_CONV THENC REWRITE_CONV[ADD_0];;
+
+let DIMINDEX_11 = DIMINDEX_CONV `dimindex (:11)`;;
+
+let compress_d11_avx2 = new_definition
+  `compress_d11_avx2 (a:16 word) : 16 word =
+   word_and
+    (word_subword
+      (word_add
+        (word_ushr
+          (word_mul
+            (word_sx
+              (word_sub
+                (word_subword (word_mul (word_sx (word_shl a 3)) (word 20159) : 32 word) (16,16) : 16 word)
+                (word_ushr
+                  (word_and (word_not (word_mul a (word 30200)))
+                    (word_sub (word_mul a (word 30200))
+                      (word_add a (word 36))))
+                  15)))
+            (word 8192) : 32 word)
+          14)
+        (word 1) : 32 word)
+      (1,16) : 16 word)
+    (word 2047)`;; 
+
+let WORD_AND_2047 = WORD_BLAST `word_and (x : 16 word) (word 2047) = word_zx (word_subword x (0,11) : 11 word) : 16 word`;;
+REWRITE_RULE [WORD_AND_2047] compress_d11_avx2
+
+let MULADD_2048_JOIN = prove(`word_add (word_mul (word_sx (word_zx (x : 11 word) : 16 word) : 32 word) (word 1))
+   (word_mul (word_sx (word_zx (y : 11 word) : 16 word) : 32 word) (word 2048)) = word_zx (word_join y x : 22 word) : 32 word`,
+  BITBLAST_TAC);;
+
+let DECOMPRESS_MULADD_2048_JOIN = prove(`((word_add:(32)word->(32)word->(32)word)
+            ((word_mul:(32)word->(32)word->(32)word)
+             ((word_sx:(16)word->(32)word)
+             ((compress_d11_avx2:(16)word->(16)word) x))
+            ((word:num->(32)word) 1))
+           ((word_mul:(32)word->(32)word->(32)word)
+            ((word_sx:(16)word->(32)word)
+            ((compress_d11_avx2:(16)word->(16)word) y))
+           ((word:num->(32)word) 2048))) = 
+    word_zx (word_join (word_subword (compress_d11_avx2 y) (0,11) : 11 word) 
+                       (word_subword (compress_d11_avx2 x) (0,11) : 11 word) : 22 word) : 32 word`,
+  REWRITE_TAC [compress_d11_avx2; WORD_AND_2047; MULADD_2048_JOIN; WORD_BLAST 
+    `!x:11 word. word_subword (word_zx x : 16 word) (0,11) : 11 word = x`]);;
+
+let WORD_SUBWORD_USHR_HIGH_64 = REWRITE_RULE[DIMINDEX_CONV `dimindex(:64)`]
+  (INST_TYPE [`:64`,`:N`] WORD_SUBWORD_USHR_HIGH);;  
+
+let DECOMPRESS_D11_CORRECT = prove(`!(x : 16 word). val x < 3329 ==> compress_d11 x = word_subword (compress_d11_avx2 x) (0,11)`,
+  let CORE = prove(`!(x : num). x < 3329 ==> compress_d11 (word x) = word_subword (compress_d11_avx2 (word x)) (0,11)`,
+    REWRITE_TAC[compress_d11; compress_d11_avx2] THEN
+    BRUTE_FORCE_WITH (CONV_TAC(WORD_REDUCE_CONV THENC NUM_REDUCE_CONV))) in
+  GEN_TAC THEN DISCH_TAC THEN
+  MP_TAC(SPEC `val(x:16 word)` CORE) THEN
+  ASM_REWRITE_TAC[WORD_VAL]);;
+ 
+type asm_info = { label: string; thm: thm; comp: string; addr: term; rhs: term };;
+
+let COMBINE_WBYTES_176_TAC : tactic = fun (asl,w) ->
+  let get_comp_addr_rhs tm =
+    try let l = lhand tm and r = rand tm in
+        let rd = rator l in
+        let comp = snd(dest_binary ":>" (rand rd)) in
+        let cname = fst(dest_const(rator comp)) in
+        {label=""; thm=TRUTH; comp=cname; addr=rand comp; rhs=r}
+    with _ -> {label=""; thm=TRUTH; comp=""; addr=`T`; rhs=`T`} in
+  let get_base_offset addr =
+    try let args = snd(strip_comb addr) in
+        (hd args, Num.int_of_num(dest_numeral (rand (hd(tl args)))))
+    with _ -> (addr, 0) in
+  let mk_info s th =
+    let i = get_comp_addr_rhs (concl th) in
+    {i with label=s; thm=th} in
+  let asms = map (fun a -> mk_info (fst a) (snd a)) asl in
+  let b128s = filter (fun i -> i.comp = "bytes128") asms in
+  let b32s  = filter (fun i -> i.comp = "bytes32") asms in
+  let b16s  = filter (fun i -> i.comp = "bytes16") asms in
+  let addr_matches base tgt i =
+    let p = get_base_offset i.addr in fst p = base && snd p = tgt in
+  let rec find_triple = function
+    | [] -> failwith "COMBINE_WBYTES_176_TAC: no matching triple"
+    | i128::rest ->
+      let p = get_base_offset i128.addr in
+      let base = fst p and off = snd p in
+      (try
+        let i32 = find (addr_matches base (off+16)) b32s in
+        let i16 = find (addr_matches base (off+20)) b16s in
+        [i128; i32; i16]
+      with _ -> find_triple rest) in
+  let trip = find_triple b128s in
+  let i128 = el 0 trip and i32 = el 1 trip and i16 = el 2 trip in
+  let s_tm = rand(lhand(concl i128.thm)) in
+  let lemma = INST [i128.addr,`a:int64`; s_tm,`s:x86state`;
+                    i128.rhs,`x0:128 word`;
+                    i32.rhs,`x1:32 word`;
+                    i16.rhs,`x2:16 word`] READ_MEMORY_WBYTES_MERGE_128_32_16 in
+  let lemma' = CONV_RULE(DEPTH_CONV(CHANGED_CONV
+    (REWRITE_CONV[WORD_ADD_ASSOC_CONSTS] THENC NUM_REDUCE_CONV))) lemma in
+  let result = MP (MP (MP lemma' i128.thm) i32.thm) i16.thm in
+  let drop_thms = [i128.thm; i32.thm; i16.thm] in
+  let asl' = filter (fun (_,th) -> not (mem th drop_thms)) asl in  
+  ASSUME_TAC result (asl',w);;
+
+let REWRITE_COMPRESS =
+   let derive_instance thm tm =
+     let thm' = PART_MATCH rand thm tm in
+      MP thm' (EQT_ELIM(NUM_REDUCE_CONV (fst(dest_imp(concl thm')))))
+   in   
+    (UNDISCH_THEN (`forall i. i < 256 ==> val (EL i (inlist : (16 word) list)) < 3329`) (fun thm -> 
+     RULE_ASSUM_TAC (CONV_RULE (TOP_DEPTH_CONV (COND_REWRITE_CONV (derive_instance thm) (GSYM DECOMPRESS_D11_CORRECT))))
+     THEN ASSUME_TAC thm
+    ));;
+
+let SIMPLIFY_WORD_ADD = RULE_ASSUM_TAC (CONV_RULE (ONCE_DEPTH_CONV (COND_REWRITE_CONV WORD_BLAST WORD_ADD_OR)));;
+
+let MLKEM_POLY_COMPRESS_D11_CORRECT = prove(
+  `!r a data (inlist:(16 word) list) pc.
+      LENGTH inlist = 256 /\
+      aligned 32 a /\
+      aligned 32 data /\
+      ALL (nonoverlapping (r, 352))
+          [(word pc, LENGTH mlkem_poly_compress_d11_tmc); (a, 512); (data, 64)]
+      ==> ensures x86
+           (\s. bytes_loaded s (word pc) (BUTLAST mlkem_poly_compress_d11_tmc) /\
+                read RIP s = word pc /\
+                C_ARGUMENTS [r; a; data] s /\
+                read (memory :> bytes(data, 64)) s =
+                  num_of_wordlist ((MAP iword compress_d11_data): (8 word) list) /\
+                read (memory :> bytes(a, 512)) s = num_of_wordlist inlist /\
+                (!i. i < 256 ==> &0 <= ival (EL i inlist) /\ ival (EL i inlist) <= &3328))
+           (\s. read RIP s = word (pc + 2120) /\
+                read (memory :> bytes(r, 352)) s = num_of_wordlist (MAP compress_d11 inlist))
+           (MAYCHANGE [events] ,,
+            MAYCHANGE [memory :> bytes(r, 352)] ,,
+            MAYCHANGE [RIP] ,, MAYCHANGE [RAX] ,,
+            MAYCHANGE [ZMM0; ZMM1; ZMM2; ZMM3; ZMM4; ZMM5; ZMM6; ZMM7; ZMM8; ZMM9; ZMM10; ZMM11])`,
+
+  MAP_EVERY X_GEN_TAC
+    [`r:int64`; `a:int64`; `data:int64`; `inlist:(16 word) list`; `pc:num`] THEN
+  CONV_TAC LENGTH_SIMPLIFY_CONV THEN
+  REWRITE_TAC[MAYCHANGE_REGS_AND_FLAGS_PERMITTED_BY_ABI; C_ARGUMENTS;
+              NONOVERLAPPING_CLAUSES; ALL] THEN
+  DISCH_THEN(REPEAT_TCL CONJUNCTS_THEN ASSUME_TAC) THEN
+  ENSURES_INIT_TAC "s0" THEN
+
+  (* Move to 256-bit granular preconditions for input array *)
+  UNDISCH_TAC `read(memory :> bytes(a,512)) (s0 : x86state) = num_of_wordlist(inlist: (16 word) list)` THEN
+  GEN_REWRITE_TAC (LAND_CONV o RAND_CONV o RAND_CONV) [GSYM LIST_OF_SEQ_EQ_SELF] THEN
+  ASM_REWRITE_TAC[] THEN
+  CONV_TAC(LAND_CONV(RAND_CONV(RAND_CONV LIST_OF_SEQ_CONV))) THEN
+  REWRITE_TAC[] THEN
+  REPLICATE_TAC 4
+   (GEN_REWRITE_TAC (LAND_CONV o ONCE_DEPTH_CONV)
+         [GSYM NUM_OF_PAIR_WORDLIST]) THEN
+  REWRITE_TAC[pair_wordlist] THEN
+  CONV_TAC(LAND_CONV BYTES_EQ_NUM_OF_WORDLIST_EXPAND_CONV) THEN
+  REWRITE_TAC[GSYM BYTES256_WBYTES] THEN 
+  REPEAT STRIP_TAC THEN
+
+  (* Move to 256-bit granular precondition for constant array *)
+  UNDISCH_TAC
+   `read(memory :> bytes(data,64)) s0 = num_of_wordlist ((MAP iword compress_d11_data) : (8 word) list)` THEN
+  REWRITE_TAC [compress_d11_data; MAP] THEN
+  REPLICATE_TAC 5 (GEN_REWRITE_TAC (LAND_CONV o ONCE_DEPTH_CONV)
+                   [GSYM NUM_OF_PAIR_WORDLIST]) THEN
+  REWRITE_TAC[pair_wordlist] THEN CONV_TAC WORD_REDUCE_CONV THEN
+  CONV_TAC(LAND_CONV BYTES_EQ_NUM_OF_WORDLIST_EXPAND_CONV) THEN
+  REWRITE_TAC[GSYM BYTES256_WBYTES] THEN STRIP_TAC THEN
+
+  SUBGOAL_THEN `!i. i < 256 ==> val (EL i (inlist:(16 word) list)) < 3329` ASSUME_TAC THENL [
+    REPEAT STRIP_TAC THEN
+    FIRST_X_ASSUM(MP_TAC o SPEC `i:num`) THEN ASM_REWRITE_TAC[] THEN
+    REWRITE_TAC[IVAL_VAL; DIMINDEX_16; bitval; BIT_VAL] THEN
+    MP_TAC(ISPEC `EL i (inlist:(16 word) list)` VAL_BOUND) THEN
+    REWRITE_TAC[DIMINDEX_16] THEN ARITH_TAC;
+    ALL_TAC] THEN
+
+  (*** Symbolic execution ***)
+  MAP_EVERY (fun n -> X86_STEPS_TAC MLKEM_POLY_COMPRESS_D11_TMC_EXEC [n] THEN SIMD_SIMPLIFY_TAC 
+    [GSYM WORD_SUBWORD_USHR_HIGH_64; GSYM WORD_SUBWORD_USHR_64; GSYM WORD_JOIN_AND_TYBIT0; GSYM WORD_JOIN_NOT_TYBIT0; compress_d11_avx2;
+     GSYM DECOMPRESS_MULADD_2048_JOIN; GSYM (CONV_RULE NUM_REDUCE_CONV BYTES128_JOIN); GSYM WORD_ZX_128_256_128; GSYM WORD_64_SUB_8_8_JOIN_16]) (1 -- 389) THEN
+
+  ENSURES_FINAL_STATE_TAC THEN ASM_REWRITE_TAC[] THEN
+
+  RULE_ASSUM_TAC (REWRITE_RULE [WORD_ADD_0]) THEN
+  DISCARD_MATCHING_ASSUMPTIONS [`read ymm s = (t : 256 word)`] THEN
+
+  REWRITE_COMPRESS THEN 
+  SIMPLIFY_WORD_ADD THEN
+
+  REPEAT (COMBINE_WBYTES_176_TAC) THEN
+  
+  SUBGOAL_THEN `LENGTH (MAP compress_d11 (inlist : (16 word) list)) = 256` ASSUME_TAC THENL [ASM_SIMP_TAC [LENGTH_MAP]; ALL_TAC] THEN 
+  MAP_EVERY (fun i -> SUBGOAL_THEN (subst [mk_small_numeral (16 * i), `i: num`] `LENGTH (SUB_LIST (i, 16) (MAP compress_d11 (inlist : (16 word) list))) = 16`) ASSUME_TAC
+      THENL [ASM_REWRITE_TAC [LENGTH_SUB_LIST] THEN NUM_REDUCE_TAC; ALL_TAC]) (0 -- 15) THEN
+            
+  IMP_REWRITE_TAC [NUM_OF_WORDLIST_SPLIT_11_256] THEN
+  CONV_TAC (ONCE_DEPTH_CONV LIST_OF_SEQ_CONV) THEN
+  REWRITE_TAC [MAP; o_DEF] THEN
+  CONV_TAC(BYTES_EQ_NUM_OF_WORDLIST_EXPAND_CONV) THEN
+  ASM_REWRITE_TAC [] THEN
+  DISCARD_MATCHING_ASSUMPTIONS [`read c s = (t : N word)`] THEN
+  REPEAT CONJ_TAC THEN
+
+  REWRITE_TAC [WORD_PACKED_EQ_D11] THEN
+  CONV_TAC (EXPAND_CASES_CONV THENC NUM_REDUCE_CONV) THEN
+  TRY (IMP_REWRITE_TAC WORD_SUBWORD_NUM_OF_WORDLIST_CASES_D11) THEN
+  REPEAT CONJ_TAC THEN
+  UNDISCH_THEN `LENGTH (MAP compress_d11 (inlist : (16 word) list)) = 256` (fun th -> 
+    CONV_TAC (TOP_SWEEP_CONV (EL_SUB_LIST_CONV th)) THEN ASSUME_TAC th) THEN
+  ASM_SIMP_TAC [EL_MAP; ARITH] THEN
+  CONV_TAC WORD_BLAST
+);;
+
+let MLKEM_POLY_COMPRESS_D11_NOIBT_SUBROUTINE_CORRECT = prove(
+  `!r a data (inlist:(16 word) list) pc stackpointer returnaddress.
+      LENGTH inlist = 256 /\
+      aligned 32 a /\
+      aligned 32 data /\
+      ALL (nonoverlapping (r, 352))
+          [(word pc, LENGTH mlkem_poly_compress_d11_tmc); (a, 512); (data, 64); (stackpointer, 8)]
+      ==> ensures x86
+           (\s. bytes_loaded s (word pc) mlkem_poly_compress_d11_tmc /\
+                read RIP s = word pc /\
+                read RSP s = stackpointer /\
+                read (memory :> bytes64 stackpointer) s = returnaddress /\
+                C_ARGUMENTS [r; a; data] s /\
+                read (memory :> bytes(data, 64)) s =
+                  num_of_wordlist ((MAP iword compress_d11_data): (8 word) list) /\
+                read (memory :> bytes(a, 512)) s = num_of_wordlist inlist /\
+                (!i. i < 256 ==> &0 <= ival (EL i inlist) /\ ival (EL i inlist) <= &3328))
+           (\s. read RIP s = returnaddress /\
+                read RSP s = word_add stackpointer (word 8) /\
+                read (memory :> bytes(r, 352)) s = num_of_wordlist (MAP compress_d11 inlist))
+           (MAYCHANGE [RSP] ,,
+            MAYCHANGE_REGS_AND_FLAGS_PERMITTED_BY_ABI ,,
+            MAYCHANGE [memory :> bytes(r, 352)])`,
+  X86_PROMOTE_RETURN_NOSTACK_TAC mlkem_poly_compress_d11_tmc
+    MLKEM_POLY_COMPRESS_D11_CORRECT);;
+
+let MLKEM_POLY_COMPRESS_D11_SUBROUTINE_CORRECT = prove(
+  `!r a data (inlist:(16 word) list) pc stackpointer returnaddress.
+      LENGTH inlist = 256 /\
+      aligned 32 a /\
+      aligned 32 data /\
+      ALL (nonoverlapping (r, 352))
+          [(word pc, LENGTH mlkem_poly_compress_d11_mc); (a, 512); (data, 64); (stackpointer, 8)]
+      ==> ensures x86
+           (\s. bytes_loaded s (word pc) mlkem_poly_compress_d11_mc /\
+                read RIP s = word pc /\
+                read RSP s = stackpointer /\
+                read (memory :> bytes64 stackpointer) s = returnaddress /\
+                C_ARGUMENTS [r; a; data] s /\
+                read (memory :> bytes(data, 64)) s =
+                  num_of_wordlist ((MAP iword compress_d11_data): (8 word) list) /\
+                read (memory :> bytes(a, 512)) s = num_of_wordlist inlist /\
+                (!i. i < 256 ==> &0 <= ival (EL i inlist) /\ ival (EL i inlist) <= &3328))
+           (\s. read RIP s = returnaddress /\
+                read RSP s = word_add stackpointer (word 8) /\
+                read (memory :> bytes(r, 352)) s = num_of_wordlist (MAP compress_d11 inlist))
+           (MAYCHANGE [RSP] ,,
+            MAYCHANGE_REGS_AND_FLAGS_PERMITTED_BY_ABI ,,
+            MAYCHANGE [memory :> bytes(r, 352)])`,
+  MATCH_ACCEPT_TAC(ADD_IBT_RULE MLKEM_POLY_COMPRESS_D11_NOIBT_SUBROUTINE_CORRECT));;
